introduce weakest precondition in the right form

HeapLang/State.thy
@@ -7,86 +7,99 @@ text \<open> State specific definitions and lemmata;
   based on \<^url>\<open>https://gitlab.mpi-sws.org/iris/iris/-/blob/master/iris_heap_lang/lang.v\<close> \<close>
 
 (* The state: heaps of val options, with None representing deallocated locations. *)
-datatype state = State (heap: "(loc,val option) map") (used_proph_id: "proph_id set")
+datatype state = State (heap: "(loc,val option) fmap") (used_proph_id: "proph_id fset")
 
-definition state_upd_heap :: "((loc,val option) map \<Rightarrow> (loc,val option) map) \<Rightarrow> state \<Rightarrow> state" where
+definition state_upd_heap :: "((loc,val option) fmap \<Rightarrow> (loc,val option) fmap) \<Rightarrow> state \<Rightarrow> state" where
   "state_upd_heap f \<sigma> = State (f (heap \<sigma>)) (used_proph_id \<sigma>)"
 
-definition state_upd_used_proph_id :: "(proph_id set \<Rightarrow> proph_id set) \<Rightarrow> state \<Rightarrow> state" where
+definition state_upd_used_proph_id :: "(proph_id fset \<Rightarrow> proph_id fset) \<Rightarrow> state \<Rightarrow> state" where
   "state_upd_used_proph_id f \<sigma> = State (heap \<sigma>) (f (used_proph_id \<sigma>))"
 
-fun heap_array :: "loc \<Rightarrow> val list \<Rightarrow> (loc, val option) map" where
-  "heap_array l [] = Map.empty"
-| "heap_array l (v#vs) = (heap_array (l+\<^sub>\<iota>1) vs)(l\<mapsto>Some v)"
+fun heap_array :: "loc \<Rightarrow> val list \<Rightarrow> (loc, val option) fmap" where
+  "heap_array l [] = fmempty"
+| "heap_array l (v#vs) = fmupd l (Some v) (heap_array (l+\<^sub>\<iota>1) vs)"
   
-lemma heap_array_singleton: "heap_array l [v] = [l\<mapsto>Some v]" by simp
+lemma heap_array_singleton: "heap_array l [v] = fmupd l (Some v) fmempty" by simp
 
-lemma heap_array_dom: "dom (heap_array l vs) = {l..< (l +\<^sub>\<iota> int (length vs))}"
+lemma heap_array_dom: "fmdom (heap_array l vs) = Abs_fset {l ..< (l +\<^sub>\<iota> int (length vs))}"
 proof (induction vs arbitrary: l)
+  case Nil
+  then show ?case by (auto simp: loc_add_0 bot_fset.abs_eq)
+next
   case (Cons a vs)
-  have "dom (heap_array l (a # vs)) = insert l (dom (heap_array (l+\<^sub>\<iota>1) vs))" by simp
-  also have "... = insert l {(l+\<^sub>\<iota>1)..< ((l+\<^sub>\<iota>1) +\<^sub>\<iota> int (length vs))}" 
+  have "fmdom (heap_array l (a # vs)) = finsert l (fmdom (heap_array (l+\<^sub>\<iota>1) vs))" by simp
+  then have "fset (fmdom (heap_array l (a # vs))) = insert l (fset (fmdom (heap_array (l+\<^sub>\<iota>1) vs)))"
+    by simp
+  also have "... = insert l (fset (Abs_fset {(l+\<^sub>\<iota>1)..< ((l+\<^sub>\<iota>1) +\<^sub>\<iota> int (length vs))}))" 
     using Cons by simp
-  also have "... = {l} \<union> {(l+\<^sub>\<iota>1)..< ((l+\<^sub>\<iota>1) +\<^sub>\<iota> int (length vs))}" 
-      by simp
-  also have "... = ({l..<(l+\<^sub>\<iota>1)} \<union>
-    {(l+\<^sub>\<iota>1)..<((l+\<^sub>\<iota>1) +\<^sub>\<iota> int (length vs))})" using less_eq_loc_def loc_add_def less_loc_def loc.expand
-    by fastforce
+  also have "... = insert l {(l+\<^sub>\<iota>1)..< ((l+\<^sub>\<iota>1) +\<^sub>\<iota> int (length vs))}"
+    using Abs_fset_inverse finite_atLeastLessThan_loc by blast
+  also have "... = {l} \<union> {(l+\<^sub>\<iota>1)..< ((l+\<^sub>\<iota>1) +\<^sub>\<iota> int (length vs))}"
+    by simp
+  also have "... = {l..<(l+\<^sub>\<iota>1)} \<union> {(l+\<^sub>\<iota>1)..<((l+\<^sub>\<iota>1) +\<^sub>\<iota> int (length vs))}" 
+    using less_eq_loc_def loc_add_def less_loc_def loc.expand finite_atLeastLessThan_int by auto
   also have "... = ({l..<(l+\<^sub>\<iota>1)} \<union> {(l+\<^sub>\<iota>1)..<(l+\<^sub>\<iota>(1 + int (length vs)))})" by (simp add: loc_add_assoc)
   also have "... = ({l..<(l+\<^sub>\<iota>1)} \<union> {(l+\<^sub>\<iota>1)..<(l+\<^sub>\<iota> int (length (a#vs)))})" by simp
   also have "... = {l..<(l +\<^sub>\<iota> int (length (a#vs)))}" 
     by (auto simp: loc_add_def loc.expand less_eq_loc_def ivl_disj_un(17))
-  finally show ?case .
-qed (simp add: loc_add_0)
+  finally have "Abs_fset (fset (fmdom (heap_array l (a # vs)))) = Abs_fset {l..<(l +\<^sub>\<iota> int (length (a#vs)))}"
+    by simp
+  then show ?case unfolding fset_inverse .
+qed 
 
-lemma heap_array_shift: "heap_array l vs k = heap_array (l+\<^sub>\<iota>n) vs (k+\<^sub>\<iota>n)"
+lemma heap_array_shift: "fmlookup (heap_array l vs) k = fmlookup (heap_array (l+\<^sub>\<iota>n) vs) (k+\<^sub>\<iota>n)"
 proof (induction vs arbitrary: l k)
   case (Cons a vs)
   show ?case apply (simp; rule impI; rule conjI) using loc_add_def apply (simp_all add: loc.expand) 
     using Cons using loc_add_def loc.expand apply blast
-    by (metis add.assoc add.left_commute loc_add_assoc local.Cons)
+    by (smt (verit) loc.sel local.Cons)
 qed (simp)
 
-lemma heap_array_cons_shift: "(heap_array l vs k = Some w) \<Longrightarrow> (heap_array l (v#vs) (k+\<^sub>\<iota>1) = Some w)"
+lemma heap_array_cons_shift: "(fmlookup (heap_array l vs) k = Some w) \<Longrightarrow> 
+  (fmlookup (heap_array l (v#vs)) (k+\<^sub>\<iota>1) = Some w)"
 proof -
-  assume assm: "heap_array l vs k = Some w"
-  hence "k \<in> dom (heap_array l vs)" by blast
-  with heap_array_dom[of l vs] have "l\<noteq>k+\<^sub>\<iota>1" using loc_add_def less_eq_loc_def by auto
-  with assm show "heap_array l (v#vs) (k+\<^sub>\<iota>1) = Some w" unfolding loc_add_def apply simp 
+  assume assm: "fmlookup (heap_array l vs) k = Some w"
+  hence "k |\<in>| fmdom (heap_array l vs)" by (rule fmdomI)
+  then have "k \<in> {l ..< (l +\<^sub>\<iota> int (length vs))}" unfolding heap_array_dom
+    by (simp add: eq_onp_same_args fmember.abs_eq)
+  then have "l\<noteq>k+\<^sub>\<iota>1"  using less_eq_loc_def loc_add_def by force
+  with assm show "fmlookup (heap_array l (v#vs)) (k+\<^sub>\<iota>1) = Some w" unfolding loc_add_def apply simp 
   using heap_array_shift loc_add_def by fastforce
 qed
 
-lemma heap_array_elements: "heap_array l vs k = Some (Some w) \<Longrightarrow> w \<in> set vs"
+lemma heap_array_elements: "fmlookup (heap_array l vs) k = Some (Some w) \<Longrightarrow> w \<in> set vs"
 proof (induction vs arbitrary: l k)
   case (Cons a vs)
-  then show ?case by (metis fun_upd_apply heap_array.simps(2) in_set_member member_rec(1) option.inject)
+  then show ?case by (metis fmupd_lookup heap_array.simps(2) in_set_member member_rec(1) option.inject)
 qed (simp)
 
-lemma heap_array_step: "\<lbrakk>heap_array l (v#vs) k = Some w; l\<noteq>k\<rbrakk> \<Longrightarrow> heap_array l vs (k+\<^sub>\<iota>(-1)) = Some w"
+lemma heap_array_step: "\<lbrakk>fmlookup (heap_array l (v#vs)) k = Some w; l\<noteq>k\<rbrakk> \<Longrightarrow> 
+  fmlookup (heap_array l vs) (k+\<^sub>\<iota>(-1)) = Some w"
 proof (induction vs arbitrary: l k v)
   case (Cons a vs)
-  from Cons(3) have "heap_array l (v # a # vs) k = heap_array (l+\<^sub>\<iota>1) (a#vs) k" by simp
-  with Cons(2) have step: "heap_array (l+\<^sub>\<iota>1) (a#vs) k = Some w" by simp
+  from Cons(3) have "fmlookup (heap_array l (v # a # vs)) k = fmlookup (heap_array (l+\<^sub>\<iota>1) (a#vs)) k" 
+    by simp
+  with Cons(2) have step: "fmlookup (heap_array (l+\<^sub>\<iota>1) (a#vs)) k = Some w" by simp
   then show ?case proof (cases "(l+\<^sub>\<iota>1=k)")
     case True
     with step have "w=Some a" by simp
     with True show ?thesis unfolding loc_add_def by auto
   next
     case False
-    from Cons(3) have "heap_array l (a # vs) (k +\<^sub>\<iota> - 1) = heap_array (l+\<^sub>\<iota>1) vs (k +\<^sub>\<iota> - 1)"
+    from Cons(3) have "fmlookup (heap_array l (a # vs)) (k +\<^sub>\<iota> - 1) = fmlookup (heap_array (l+\<^sub>\<iota>1) vs) (k +\<^sub>\<iota> - 1)"
       using loc_add_def False by force
     with Cons(1)[OF step False] show ?thesis by simp
   qed
 qed (simp)
 
 (* Due to nth being defined as primrec, this can't be an iff but only a one sided implication. *)
-lemma heap_array_lookup: "((heap_array l vs) k = Some (Some ow)) \<Longrightarrow>
+lemma heap_array_lookup: "(fmlookup (heap_array l vs) k = Some (Some ow)) \<Longrightarrow>
   (\<exists>j w. 0 \<le> j \<and> k = l +\<^sub>\<iota> j \<and> vs!(nat j) = w \<and> w=ow)"
 proof (induction vs arbitrary: k)
   case (Cons a vs)
   then show ?case proof (cases "l=k")
     case True
-    hence "heap_array l (a#vs) k = Some (Some a)" by simp
+    hence "fmlookup (heap_array l (a#vs)) k = Some (Some a)" by simp
     with Cons(2) have "ow = a" by simp
     moreover from True have "k=l+\<^sub>\<iota>0 \<and> (0::int)\<le>0 \<and> (a#vs)!(nat 0) = a" by (simp add: loc_add_0)
     ultimately show ?thesis by blast
@@ -100,22 +113,23 @@ proof (induction vs arbitrary: k)
   qed
 qed (simp)
 
-lemma state_array_map_disjoint: "(\<forall>i. (0\<le>i \<longrightarrow> (nat i < length vs) \<longrightarrow> h (l+\<^sub>\<iota>i) = None))
-  \<Longrightarrow> dom (heap_array l vs) \<inter> dom h = {}"
+lemma state_array_map_disjoint: "(\<forall>i. (0\<le>i \<longrightarrow> (nat i < length vs) \<longrightarrow> fmlookup h (l+\<^sub>\<iota>i) = None))
+  \<Longrightarrow> fmdom (heap_array l vs) |\<inter>| fmdom h = {||}"
 proof
-  assume assm: "\<forall>i\<ge>0. nat i < length vs \<longrightarrow> h (l +\<^sub>\<iota> i) = None"
-  from assm have "\<forall>i\<ge>0. nat i < length vs \<longrightarrow> (l +\<^sub>\<iota> i) \<notin> dom h" by fastforce
-  hence "\<forall>i \<in> {0..<(int (length vs))}. (l +\<^sub>\<iota> i) \<notin> dom h" by fastforce
-  hence "\<forall>l' \<in> {(l +\<^sub>\<iota> i) | i. i \<in> {0..<(int (length vs))} }. l' \<notin> dom h" by blast
-  hence "\<forall>l' \<in> {l..<(l +\<^sub>\<iota> int (length vs))}. l' \<notin> dom h" using loc_ranges by blast
-  hence "{l..<(l +\<^sub>\<iota> int (length vs))} \<inter> dom h = {}" by auto
-  with heap_array_dom show "dom (heap_array l vs) \<inter> dom h \<subseteq> {}" by auto
+  assume assm: "\<forall>i\<ge>0. nat i < length vs \<longrightarrow> fmlookup h (l +\<^sub>\<iota> i) = None"
+  from assm have "\<forall>i\<ge>0. nat i < length vs \<longrightarrow> (l +\<^sub>\<iota> i) |\<notin>| fmdom h" by fastforce
+  hence "\<forall>i \<in> {0..<(int (length vs))}. (l +\<^sub>\<iota> i) |\<notin>| fmdom h" by fastforce
+  hence "\<forall>l' \<in> {(l +\<^sub>\<iota> i) | i. i \<in> {0..<(int (length vs))} }. l' |\<notin>| fmdom h" by blast
+  hence "\<forall>l' \<in> {l..<(l +\<^sub>\<iota> int (length vs))}. l' |\<notin>| fmdom h" using loc_ranges by blast
+  hence "Abs_fset {l..<(l +\<^sub>\<iota> int (length vs))} |\<inter>| fmdom h = {||}"
+    by (metis all_not_fin_conv eq_onp_same_args finite_atLeastLessThan_loc finter_iff fmember.abs_eq)
+  with heap_array_dom show "fmdom (heap_array l vs) |\<inter>| fmdom h |\<subseteq>| {||}" by auto
 qed (simp)
 
 definition state_init_heap :: "loc \<Rightarrow> nat \<Rightarrow> val \<Rightarrow> state \<Rightarrow> state" where
-  "state_init_heap l n v \<sigma> = state_upd_heap (\<lambda>h. h ++ heap_array l (replicate n v)) \<sigma>"
+  "state_init_heap l n v \<sigma> = state_upd_heap (\<lambda>h. h ++\<^sub>f heap_array l (replicate n v)) \<sigma>"
 
-lemma state_init_heap_singleton: "state_init_heap l 1 v \<sigma> = state_upd_heap (\<lambda>h. h(l\<mapsto>Some v)) \<sigma>"
+lemma state_init_heap_singleton: "state_init_heap l 1 v \<sigma> = state_upd_heap (\<lambda>h. fmupd l (Some v) h) \<sigma>"
 unfolding state_init_heap_def by simp
 
 inductive head_step :: "expr \<Rightarrow> state \<Rightarrow> observation list \<Rightarrow> expr \<Rightarrow> state \<Rightarrow> expr list \<Rightarrow> bool" 
@@ -137,27 +151,27 @@ inductive head_step :: "expr \<Rightarrow> state \<Rightarrow> observation list 
 | CaseLS: "(Case (Val(InjLV v)) e1 e2) \<sigma> [] \<Rightarrow>\<^sub>h (App e1 (Val v)) \<sigma> []"
 | CaseRS: "(Case (Val(InjRV v)) e1 e2) \<sigma> [] \<Rightarrow>\<^sub>h (App e2 (Val v)) \<sigma> []"
 | ForkS: "(Fork e) \<sigma> [] \<Rightarrow>\<^sub>h (Val(LitV LitUnit)) \<sigma> [e]"
-| AllocNS: "\<lbrakk>(0 < n); (\<forall> (i::int). (0 \<le> i) \<longrightarrow> (i < n) \<longrightarrow> heap \<sigma> (l +\<^sub>\<iota> i) = None)\<rbrakk> \<Longrightarrow>
+| AllocNS: "\<lbrakk>(0 < n); (\<forall> (i::int). (0 \<le> i) \<longrightarrow> (i < n) \<longrightarrow> fmlookup (heap \<sigma>) (l +\<^sub>\<iota> i) = None)\<rbrakk> \<Longrightarrow>
   (AllocN (Val(LitV(LitInt n))) (Val v)) \<sigma> [] \<Rightarrow>\<^sub>h
   (Val(LitV(LitLoc l))) (state_init_heap l (nat n) v \<sigma>) []"
-| FreeS: "heap \<sigma> l = Some v \<Longrightarrow> 
-  (Free (Val(LitV(LitLoc l)))) \<sigma> [] \<Rightarrow>\<^sub>h (Val(LitV LitUnit)) (state_upd_heap (\<lambda>h. h(l\<mapsto>None)) \<sigma>) []"
-| LoadS: "heap \<sigma> l = Some (Some v) \<Longrightarrow> (Load (Val(LitV(LitLoc l)))) \<sigma> [] \<Rightarrow>\<^sub>h (of_val v) \<sigma> []"
-| StoreS: "heap \<sigma> l = Some (Some v) \<Longrightarrow>
+| FreeS: "fmlookup (heap \<sigma>) l = Some v \<Longrightarrow> 
+  (Free (Val(LitV(LitLoc l)))) \<sigma> [] \<Rightarrow>\<^sub>h (Val(LitV LitUnit)) (state_upd_heap (\<lambda>h. fmupd l None h) \<sigma>) []"
+| LoadS: "fmlookup (heap \<sigma>) l = Some (Some v) \<Longrightarrow> (Load (Val(LitV(LitLoc l)))) \<sigma> [] \<Rightarrow>\<^sub>h (of_val v) \<sigma> []"
+| StoreS: "fmlookup (heap \<sigma>) l = Some (Some v) \<Longrightarrow>
   (Store (Val(LitV(LitLoc l))) (Val w)) \<sigma> [] \<Rightarrow>\<^sub>h
-  (Val(LitV LitUnit)) (state_upd_heap (\<lambda>h. h(l\<mapsto>Some w)) \<sigma>) []"
-| XchgS: "heap \<sigma> l = Some (Some v1) \<Longrightarrow>
+  (Val(LitV LitUnit)) (state_upd_heap (\<lambda>h. fmupd l (Some w) h) \<sigma>) []"
+| XchgS: "fmlookup (heap \<sigma>) l = Some (Some v1) \<Longrightarrow>
   (Xchg (Val(LitV(LitLoc l))) (Val v2)) \<sigma> [] \<Rightarrow>\<^sub>h
-  (Val v1) (state_upd_heap (\<lambda>h. h(l\<mapsto>Some v2)) \<sigma>) []"
+  (Val v1) (state_upd_heap (\<lambda>h. fmupd l (Some v2) h) \<sigma>) []"
    (* Crucially, this compares the same way as [EqOp]! *)
-| CmpXchgS: "\<lbrakk>heap \<sigma> l = Some (Some vl); vals_compare_safe vl v1; b = (vl = v1)\<rbrakk> \<Longrightarrow>
+| CmpXchgS: "\<lbrakk>fmlookup (heap \<sigma>) l = Some (Some vl); vals_compare_safe vl v1; b = (vl = v1)\<rbrakk> \<Longrightarrow>
   (CmpXchg (Val(LitV(LitLoc l))) (Val v1) (Val v2)) \<sigma> [] \<Rightarrow>\<^sub>h
-  (Val(PairV vl (LitV(LitBool b)))) (if b then state_upd_heap (\<lambda>h. h(l\<mapsto>Some v2)) \<sigma> else \<sigma>) []"
-| FaaS: "heap \<sigma> l = Some (Some (LitV (LitInt i1))) \<Longrightarrow>
+  (Val(PairV vl (LitV(LitBool b)))) (if b then state_upd_heap (\<lambda>h. fmupd l (Some v2) h) \<sigma> else \<sigma>) []"
+| FaaS: "fmlookup (heap \<sigma>) l = Some (Some (LitV (LitInt i1))) \<Longrightarrow>
   (FAA (Val(LitV(LitLoc l))) (Val(LitV(LitInt i2)))) \<sigma> [] \<Rightarrow>\<^sub>h
-  (Val(LitV(LitInt i1))) (state_upd_heap (\<lambda>h. h(l\<mapsto>Some (LitV (LitInt (i1 + i2))))) \<sigma>) []"
-| NewProphS: "p \<notin> used_proph_id \<sigma> \<Longrightarrow>
-  NewProph \<sigma> [] \<Rightarrow>\<^sub>h (Val(LitV(LitProphecy p))) (state_upd_used_proph_id (insert p) \<sigma>) []"
+  (Val(LitV(LitInt i1))) (state_upd_heap (\<lambda>h. fmupd l (Some (LitV (LitInt (i1 + i2)))) h) \<sigma>) []"
+| NewProphS: "p |\<notin>| used_proph_id \<sigma> \<Longrightarrow>
+  NewProph \<sigma> [] \<Rightarrow>\<^sub>h (Val(LitV(LitProphecy p))) (state_upd_used_proph_id (finsert p) \<sigma>) []"
 | ResolveS: "e \<sigma> \<kappa>s \<Rightarrow>\<^sub>h (Val v) \<sigma>' ts \<Longrightarrow>
   (Resolve e (Val(LitV(LitProphecy p))) (Val w)) \<sigma> (\<kappa>s@[(p, (v, w))]) \<Rightarrow>\<^sub>h (Val v) \<sigma>' ts"
  
@@ -297,11 +311,13 @@ next
   then show ?case by (cases Ki1) auto
 qed
 
-lemma alloc_fresh:  "(0 < n) \<Longrightarrow> finite (dom (heap \<sigma>)) \<Longrightarrow>
+lemma alloc_fresh:  "(0 < n) \<Longrightarrow>
   (AllocN ((Val(LitV(LitInt n)))) (Val v)) \<sigma> [] \<Rightarrow>\<^sub>h
-  (Val(LitV(LitLoc (fresh_locs (sorted_list_of_set (dom (heap \<sigma>))))))) (state_init_heap (fresh_locs (sorted_list_of_set (dom (heap \<sigma>)))) (nat n) v \<sigma>) []"
-  apply (rule AllocNS) using fresh_locs_fresh[of _ "(sorted_list_of_set (dom (heap \<sigma>)))"] by auto
-
+  (Val(LitV(LitLoc (fresh_locs (sorted_list_of_fset (fmdom (heap \<sigma>))))))) 
+    (state_init_heap (fresh_locs (sorted_list_of_fset (fmdom (heap \<sigma>)))) (nat n) v \<sigma>) []"
+  apply (rule AllocNS) using fresh_locs_fresh[of _ "(sorted_list_of_fset (fmdom (heap \<sigma>)))"] 
+  by (auto simp : fmdom'_alt_def fmdom'_notD)
+  
 lemma head_step_to_val: "\<lbrakk>e1 \<sigma>1 \<kappa> \<Rightarrow>\<^sub>h e2 \<sigma>2 efs; e1 \<sigma>1' \<kappa>' \<Rightarrow>\<^sub>h e2' \<sigma>2' efs'; \<exists>x. Some x = (to_val e2)\<rbrakk>
   \<Longrightarrow> \<exists>x. Some x = (to_val e2')"
   by (induction rule: head_step.induct) auto
